\documentclass[12pt,a4paper]{article}

% ----------- Packages -----------
\usepackage{amsmath, amssymb, amsthm} % Math symbols & theorems
\usepackage{enumitem} % Better lists
\usepackage{geometry} % Page layout
\usepackage{fancyhdr} % Header/footer
\usepackage{tikz}     % Diagrams
\usepackage{hyperref} % Clickable references
\usepackage{mathrsfs} % Fancy math fonts

% ----------- Page Setup -----------
\geometry{margin=1in}
\setlength{\parskip}{0.5em}
\setlength{\parindent}{0pt}
\pagestyle{fancy}
\fancyhf{}
% ----------- Header/Footer -----------
\lhead{MAT121 -- Analysis I}
\chead{Exercise sheet 1}
\rhead{Stefan du Toit}
\rfoot{\thepage}

% ----------- Theorem Environments -----------
\newtheorem{theorem}{Theorem}[section]
\newtheorem{lemma}[theorem]{Lemma}
\newtheorem{proposition}[theorem]{Proposition}
\newtheorem{corollary}[theorem]{Corollary}

\theoremstyle{definition}
\newtheorem{definition}[theorem]{Definition}
\newtheorem{example}[theorem]{Example}
\newtheorem{exercise}{Exercise}[section]

\theoremstyle{remark}
\newtheorem*{remark}{Remark}

% ----------- Custom Environments -----------
\newenvironment{solution}{\begin{proof}[Solution]}{\end{proof}}



% ==========================================
\begin{document}
\section*{5}
\subsection*{(c)}
\begin{proof}
Let \(S_n = \sum_{k=1}^{2^{n}} \frac{1}{k}\). We prove by induction on \(n \ge 1\) that
\[
S_n \le n+1.
\]

\emph{Base case \(n=1\).} Then \(S_1 = 1 + \tfrac12 = \tfrac32 \le 2 = 1+1\).

\emph{Induction step.} Assume \(S_n \le n+1\) for some \(n \ge 1\). Then
\[
S_{n+1}
= \sum_{k=1}^{2^{n+1}} \frac{1}{k}
= \sum_{k=1}^{2^{n}} \frac{1}{k} \;+\; \sum_{k=2^{n}+1}^{2^{n+1}} \frac{1}{k}
\le (n+1) \;+\; \sum_{k=2^{n}+1}^{2^{n+1}} \frac{1}{k}.
\]
For every \(k\) with \(2^{n}+1 \le k \le 2^{n+1}\), we have \(k \ge 2^{n}\), hence \(\frac{1}{k} \le \frac{1}{2^{n}}\).
There are exactly \(2^{n}\) terms in the last sum, so
\[
\sum_{k=2^{n}+1}^{2^{n+1}} \frac{1}{k} \le 2^{n} \cdot \frac{1}{2^{n}} = 1.
\]
Therefore \(S_{n+1} \le (n+1) + 1 = n+2\). This completes the induction.

Hence \(\displaystyle \sum_{k=1}^{2^{n}} \frac{1}{k} \le n+1\) for all \(n \ge 1\).
\end{proof}
\end{document}