\documentclass[12pt,a4paper]{article}

% ----------- Packages -----------
\usepackage{amsmath, amssymb, amsthm} % Math symbols & theorems
\usepackage{enumitem} % Better lists
\usepackage{geometry} % Page layout
\usepackage{fancyhdr} % Header/footer
\usepackage{tikz}     % Diagrams
\usepackage{hyperref} % Clickable references
\usepackage{mathrsfs} % Fancy math fonts

% ----------- Page Setup -----------
\geometry{margin=1in}
\setlength{\parskip}{0.5em}
\setlength{\parindent}{0pt}
\pagestyle{fancy}
\fancyhf{}
% ----------- Header/Footer -----------
\lhead{MAT121 -- Analysis I}
\chead{Exercise sheet 1}
\rhead{Stefan du Toit}
\rfoot{\thepage}

% ----------- Theorem Environments -----------
\newtheorem{theorem}{Theorem}[section]
\newtheorem{lemma}[theorem]{Lemma}
\newtheorem{proposition}[theorem]{Proposition}
\newtheorem{corollary}[theorem]{Corollary}

\theoremstyle{definition}
\newtheorem{definition}[theorem]{Definition}
\newtheorem{example}[theorem]{Example}
\newtheorem{exercise}{Exercise}[section]

\theoremstyle{remark}
\newtheorem*{remark}{Remark}

% ----------- Custom Environments -----------
\newenvironment{solution}{\begin{proof}[Solution]}{\end{proof}}



% ==========================================
\begin{document}

% Given: (a_n) real, and b_n := a_{n+1} - a_n \to 0.
% Claim: a_n / n \to 0.

\begin{lemma}
Let $(a_n)_{n\in\mathbb{N}}$ be a real sequence and $b_n := a_{n+1}-a_n \to 0$.
Then
\[
\frac{a_n}{n}\xrightarrow[n\to\infty]{} 0.
\]
\end{lemma}

\begin{proof}
By telescoping, for $n\ge 1$,
\[
a_n - a_0 = \sum_{j=0}^{n-1} (a_{j+1}-a_j) = \sum_{j=0}^{n-1} b_j.
\]
Dividing by $n$ gives
\[
\frac{a_n}{n} = \frac{a_0}{n} + \frac{1}{n}\sum_{j=0}^{n-1} b_j.
\]
Clearly $\frac{a_0}{n}\to 0$. Set
\[
m_n := \frac{1}{n}\sum_{j=0}^{n-1} b_j.
\]
We show $m_n\to 0$.

Fix $\varepsilon>0$. Since $b_n\to 0$, there exists $J\in\mathbb{N}$ such that
\[
|b_j|<\varepsilon \quad \text{for all } j\ge J.
\]
For $n>J$,
\[
\left|\frac{1}{n}\sum_{j=0}^{n-1} b_j\right|
\le \frac{1}{n}\sum_{j=0}^{J-1} |b_j| \;+\; \frac{1}{n}\sum_{j=J}^{n-1} |b_j|
\le \frac{1}{n}\sum_{j=0}^{J-1} |b_j| \;+\; \frac{n-J}{n}\,\varepsilon.
\]
Let $C := \sum_{j=0}^{J-1} |b_j| < \infty$. Choose $N$ so that $\frac{C}{n}<\varepsilon$ for all $n\ge N$.
Then for all $n\ge \max\{N,J+1\}$,
\[
\left|\frac{1}{n}\sum_{j=0}^{n-1} b_j\right|
\le \frac{C}{n} + \frac{n-J}{n}\,\varepsilon
< \varepsilon + \varepsilon
= 2\varepsilon.
\]
Since $\varepsilon>0$ was arbitrary, $m_n\to 0$. Together with $\frac{a_0}{n}\to 0$ we conclude
\[
\frac{a_n}{n} = \frac{a_0}{n} + m_n \xrightarrow[n\to\infty]{} 0.
\]
\end{proof}



\end{document}